Refactor to split memory from the configuration

src/Memory.v
@@ -1,8 +1,14 @@
 From Coq Require Import
      Arith.PeanoNat
-     Logic.FunctionalExtensionality.
+     Logic.FunctionalExtensionality
+     Lists.List
+     Lia.
 
-Require Export Heapster.Permissions.
+From Heapster Require Import
+     Utils
+     Permissions.
+
+Import ListNotations.
 
 (* Memory model *)
 Definition addr : Set := nat * nat.
@@ -41,11 +47,183 @@ Qed.
 
 Inductive Value :=
 | VNum : nat -> Value
-| VPtr : addr -> Value
-.
+| VPtr : addr -> Value.
+
 Definition mem_block := nat -> option Value.
 
 Variant logical_block :=
 | LBlock (size : nat) (bytes : mem_block) : logical_block.
 
 Definition memory := list (option logical_block).
+
+(* is the block of ptr allocated and is the offset of ptr within bounds *)
+Definition allocated (m : memory) (ptr : addr) : bool :=
+  match nth_error m (fst ptr) with
+  | Some (Some (LBlock size _)) => snd ptr <? size
+  | _ => false
+  end.
+
+(* read c at memory location ptr. ptr must be a valid location and allocated. *)
+Definition read (m : memory) (ptr : addr) : option Value :=
+  if allocated m ptr
+  then match nth_error m (fst ptr) with
+       | Some (Some (LBlock _ bytes)) => bytes (snd ptr)
+       | _ => None
+       end
+  else None.
+
+(* returns the size of the block only if ptr has offset 0 *)
+(* note if we used `allocated` here then it doesn't work for size 0 blocks... *)
+Definition sizeof (m : memory) (ptr : addr) : option nat :=
+  if snd ptr =? 0
+  then match nth_error m (fst ptr) with
+       | Some (Some (LBlock size _)) => Some size
+       | _ => None
+       end
+  else None.
+
+Definition write (m : memory) (ptr : addr) (v : Value) : option memory :=
+  if allocated m ptr
+  then match nth_error m (fst ptr) with
+       | Some (Some (LBlock size bytes)) =>
+         Some (replace_list_index
+                 m
+                 (fst ptr)
+                 (Some (LBlock size (fun o => if o =? snd ptr
+                                           then Some v
+                                           else bytes o))))
+       | _ => None
+       end
+  else None.
+
+Lemma allocated_ptr_block m b o :
+  allocated m (b, o) = true ->
+  b < length m.
+Proof.
+  unfold allocated. simpl. intros.
+  apply nth_error_Some. intro. rewrite H0 in H. inversion H.
+Qed.
+
+Lemma allocated_ptr_offset m b o size bytes :
+  allocated m (b, o) = true ->
+  nth_error m b = Some (Some (LBlock size bytes)) ->
+  o < size.
+Proof.
+  unfold allocated. simpl. intros. rewrite H0 in H.
+  rewrite <- (Bool.reflect_iff _ _ (Nat.ltb_spec0 _ _)) in H. auto.
+Qed.
+
+Lemma read_success_write m ptr v v' :
+  read m ptr = Some v ->
+  exists m', write m ptr v' = Some m'.
+Proof.
+  unfold read, write. intros.
+  destruct (allocated m ptr), (nth_error m (fst ptr));
+    try destruct o; try solve [inversion H].
+  destruct l. eexists. reflexivity.
+Qed.
+
+Lemma write_success_read_eq m m' ptr v :
+  write m ptr v = Some m' ->
+  read m' ptr = Some v.
+Proof.
+  unfold read, write. intros.
+  destruct (allocated m ptr) eqn:?, (nth_error m (fst ptr)) eqn:?;
+           try destruct o; try solve [inversion H].
+  destruct l. inversion H. clear H H1 m'. unfold allocated in *.
+  rewrite nth_error_replace_list_index_eq; [| eapply allocated_ptr_block; eauto].
+  rewrite Heqo in Heqb. clear Heqo. rewrite Heqb. rewrite Nat.eqb_refl; auto.
+Qed.
+
+Lemma write_success_read_neq m m' ptr v :
+  write m ptr v = Some m' ->
+  forall ptr', ptr <> ptr' -> read m ptr' = read m' ptr'.
+Proof.
+  destruct ptr as [b o].
+  unfold write. unfold read. simpl. intros.
+  destruct (allocated m (b, o)) eqn:?; try solve [inversion H].
+  destruct (nth_error m b) eqn:?; try solve [inversion H].
+  destruct o0 eqn:?; try solve [inversion H].
+  destruct l. inversion H; subst; clear H. destruct ptr' as [b' o']. simpl.
+  pose proof (allocated_ptr_block _ _ _ Heqb0).
+  destruct (addr_neq_cases _ _ _ _ H0).
+  - unfold allocated. simpl. erewrite nth_error_replace_list_index_neq; eauto.
+  - destruct (Nat.eq_dec b b').
+    + subst. unfold allocated. simpl. rewrite nth_error_replace_list_index_eq; auto.
+      rewrite Heqo0. destruct (o' <? size) eqn:?; auto.
+      rewrite <- Nat.eqb_neq in H1. rewrite Nat.eqb_sym. rewrite H1. auto.
+    + unfold allocated. simpl. erewrite nth_error_replace_list_index_neq; eauto.
+Qed.
+
+Lemma write_success_sizeof m m' ptr v :
+  write m ptr v = Some m' ->
+  forall ptr', sizeof m ptr' = sizeof m' ptr'.
+Proof.
+  destruct ptr as [b o].
+  unfold write. unfold read. simpl. intros.
+  destruct (allocated m (b, o)) eqn:?; try solve [inversion H].
+  destruct (nth_error m b) eqn:?; try solve [inversion H].
+  destruct o0 eqn:?; try solve [inversion H].
+  destruct l. inversion H; subst; clear H. destruct ptr' as [b' o']. simpl.
+  pose proof (allocated_ptr_block _ _ _ Heqb0).
+  unfold sizeof. simpl. destruct (o' =? 0) eqn:?; auto.
+  destruct (Nat.eq_dec b b').
+  - subst. simpl. rewrite nth_error_replace_list_index_eq; auto.
+    rewrite Heqo0. auto.
+  - erewrite nth_error_replace_list_index_neq; eauto.
+Qed.
+
+Lemma write_success_length m m' ptr v :
+  write m ptr v = Some m' ->
+  length m = length m'.
+Proof.
+  destruct ptr as [b o].
+  unfold write. unfold read. simpl. intros.
+  destruct (allocated m (b, o)) eqn:?; try solve [inversion H].
+  destruct (nth_error m b) eqn:?; try solve [inversion H].
+  destruct o0 eqn:?; try solve [inversion H].
+  destruct l. inversion H; subst; clear H.
+  pose proof (allocated_ptr_block _ _ _ Heqb0).
+  simpl. apply replace_list_index_length; auto.
+Qed.
+
+(* mem_at ptr v creates a memory which is only defined at location ptr *)
+Definition mem_at (ptr : addr) (v : Value) : memory :=
+  repeat None (fst ptr) ++ [Some (LBlock
+                                    (snd ptr + 1)
+                                    (fun o => if o =? snd ptr
+                                           then Some v
+                                           else None))].
+
+Lemma allocated_mem_at ptr v : allocated (mem_at ptr v) ptr = true.
+  destruct ptr as [b o]. unfold allocated, mem_at. simpl.
+  induction b; simpl; auto. apply Nat.ltb_lt. lia.
+Qed.
+
+Lemma nth_error_mem_at ptr v :
+  nth_error (mem_at ptr v) (fst ptr) =
+  Some (Some (LBlock
+                (snd ptr + 1)
+                (fun o => if o =? snd ptr
+                       then Some v
+                       else None))).
+Proof.
+  destruct ptr as [b o]. simpl. induction b; auto.
+Qed.
+
+Lemma read_mem_at ptr v : read (mem_at ptr v) ptr = Some v.
+Proof.
+  destruct ptr as [b o]. unfold read.
+  rewrite allocated_mem_at. rewrite nth_error_mem_at.
+  rewrite Nat.eqb_refl. reflexivity.
+Qed.
+
+Lemma write_mem_at ptr v v' : write (mem_at ptr v) ptr v' = Some (mem_at ptr v').
+Proof.
+  destruct ptr as [b o]. unfold write.
+  rewrite allocated_mem_at. rewrite nth_error_mem_at. f_equal.
+  unfold mem_at. simpl.
+  induction b; simpl; try solve [f_equal; auto].
+  do 3 f_equal. apply functional_extensionality. intros.
+  destruct (x =? o); auto.
+Qed.
