src/Utils.v
@@ -1,0 +1,69 @@
+Require Import Coq.Lists.List.
+
+Import ListNotations.
+
+Class Lens (A B:Type) : Type :=
+  {
+  lget: A -> B;
+  lput: A -> B -> A;
+  lGetPut: forall a b, lget (lput a b) = b;
+  lPutGet: forall a, lput a (lget a) = a;
+  lPutPut: forall a b b', lput (lput a b) b' = lput a b'
+  }.
+
+Fixpoint replace_list_index {A : Type} (l : list A) (n : nat) (new : A) :=
+  match l with
+  | [] => repeat new (n + 1)
+  | h :: t => match n with
+            | O => new :: t
+            | S n => h :: replace_list_index t n new
+            end
+  end.
+
+Lemma replace_list_index_length A (l : list A) n (a : A) :
+  n < length l ->
+  length l = length (replace_list_index l n a).
+Proof.
+  revert l. induction n; intros l Hl.
+  - destruct l; auto. inversion Hl.
+  - destruct l.
+    + inversion Hl.
+    + simpl in Hl. apply Lt.lt_S_n in Hl. simpl. f_equal. auto.
+Qed.
+
+Lemma nth_error_replace_list_index_neq A n n' (l : list A) (a : A) :
+  n' < length l ->
+  n <> n' ->
+  nth_error l n = nth_error (replace_list_index l n' a) n.
+Proof.
+  revert l n'.
+  induction n; intros l n' Hl Hn; (destruct l; [inversion Hl |]);
+    simpl; destruct n'; intuition.
+Qed.
+
+Lemma nth_error_replace_list_index_eq A n (l : list A) (a : A) :
+  n < length l ->
+  nth_error (replace_list_index l n a) n = Some a.
+Proof.
+  revert l. induction n; intros l Hl; (destruct l; [inversion Hl |]); simpl; auto.
+  simpl in Hl. apply Lt.lt_S_n in Hl. apply IHn; auto.
+Qed.
+
+Lemma nth_error_app_last A n (l : list A) (a : A) :
+  length l = n ->
+  nth_error (l ++ [a]) n = Some a.
+Proof.
+  revert l. induction n; intros [| l] Hl; inversion Hl; auto.
+  simpl. remember (length l0). subst. apply IHn; auto.
+Qed.
+
+Lemma nth_error_app_early A n (l : list A) (a : A) :
+  n < length l ->
+  nth_error (l ++ [a]) n = nth_error l n.
+Proof.
+  revert l. induction n; intros l Hl.
+  - destruct l; auto; inversion Hl.
+  - destruct l; auto.
+    + inversion Hl.
+    + simpl in Hl. apply Lt.lt_S_n in Hl. apply IHn; auto.
+Qed.
